lib/Lib.ByteSequence.fsti
@@ -125,3 +125,13 @@ val nat_from_intseq_le_inj:
     (requires length b1 == length b2 /\ nat_from_intseq_le b1 == nat_from_intseq_le b2)
     (ensures Seq.equal b1 b2)
     (decreases (length b1))
+
+val lemma_nat_to_from_bytes_be_preserves_value: #l:secrecy_level -> b:bytes_l l -> len:size_nat{len == length b} -> x:size_nat{x < pow2 (8 * len)} ->
+  Lemma
+  (requires (True))
+  (ensures  (nat_from_bytes_be (nat_to_bytes_be #l len x) == x))
+
+val lemma_nat_to_from_bytes_le_preserves_value: #l:secrecy_level -> b:bytes_l l -> len:size_nat{len == length b} -> x:size_nat{x < pow2 (8 * len)} ->
+  Lemma
+  (requires (True))
+  (ensures  (nat_from_bytes_le (nat_to_bytes_le #l len x) == x))
